TCSearch tactic

src/lib/TRed2.v
@@ -1,54 +1,90 @@
-From Fairness Require Import TRed.
+From Fairness Require Export Red.
+Require Import String.
+
+Variant red_class: Type := | red_class_cons: string -> red_class.
+
+Class red_db (c: red_class)
+      (A: Type)
+      (a: A) :=
+  mk_red_db {
+      red_lemma_type: Type;
+      red_lemma: red_lemma_type;
+      red_focused_type: Type;
+      red_focused: red_focused_type;
+      red_next: (_flag + red_class)%type;
+    }.
+Arguments red_db _ [_] _.
+Arguments mk_red_db _ [_] _ [_] _ [_] _ _.
+Arguments red_lemma [_ _ _] _.
+Arguments red_focused [_ _ _] _.
+Arguments red_next [_ _ _] _.
+
+Class red_db_incl (c0 c1: red_class) :=
+  mk_red_db_incl { }.
+Arguments mk_red_db_incl {_ _}.
+
+#[export] Instance red_db_incl_focus c0 c1 `{red_db_incl c0 c1}
+ A (a: A)
+  : red_db c1 a :=
+  mk_red_db _ _ (@id) a (inr c0).
+
 From Ltac2 Require Import Ltac2.
-From Ltac2 Require Option Array Ident Control Std.
+From Ltac2 Require Option Array Ident Control Std Fresh Message.
+
+Ltac2 or t0 t1 :=
+  match! 'True with
+  | True => t0 ()
+  | _ => t1 ()
+  end.
+
+Ltac2 fail () := Control.zero Match_failure.
+
+Ltac message :=
+  ltac2:(e |-
+           let e := Option.get (Ltac1.to_constr e) in
+           Message.print (Message.of_constr e))
+.
 
 Ltac2 tcsearch e :=
   let x := Array.make 1 constr:(tt: unit) in
-  match! 'True with
-  | True =>
-      let n := ident:(_TC_) in
-      ltac1:(e n|- unshelve evar (n: e);
-             [typeclasses eauto|]) (Ltac1.of_constr e) (Ltac1.of_ident n);
-      Array.set x 0 (Std.eval_unfold [(Std.VarRef n, Std.AllOccurrences)] (Control.hyp n));
-      Control.zero Match_failure
-  | _ => Array.get x 0
-  end.
+  or (fun _ =>
+        let n := Fresh.in_goal ident:(_TC_) in
+        ltac1:(e n|- unshelve evar (n: e);
+               [typeclasses eauto|]) (Ltac1.of_constr e) (Ltac1.of_ident n);
+        Array.set x 0 (Std.eval_unfold [(Std.VarRef n, Std.AllOccurrences)] (Control.hyp n));
+        fail ())
+     (fun _ => Array.get x 0)
+.
 
-Class foo_class (n: nat) := mk_foo_class {}.
-#[export] Instance foo_instance: foo_class 3 := mk_foo_class _.
+Ltac tcsearch :=
+  ltac2:(e k |-
+           let e := Option.get (Ltac1.to_constr e) in
+           let v := tcsearch e in
+           Ltac1.apply k [Ltac1.of_constr v] Ltac1.run)
+.
 
-Goal .
-  let
-
-  let (tcsearch
-
-
-Ltac2 rec _red_tac c f term k :=
-  match! c with
-  | inr ?c =>
-      (let tc := tcsearch constr:(@red_db ltac2:(@c) _ ltac2:(term)) in
-       let lem := constr:(red_lemma ltac2:(tc)) in
-       let _focused := constr:(red_focused ltac2:(tc)) in
-       let focused := (eval simpl in ltac2:(_focused)) in
-       let _next := constr:(red_next ltac2:(tc)) in
-       let next := (eval simpl in ltac2:(_next)) in
-       _red_tac next f focused (k; ltac1:(lem |- eapply lem) (Ltac1.of_constr lem)))
-  | inl ?fl =>
-      ltac1:(instantiate (f:=ltac2:(@fl))); k
-  end.
+Set Default Proof Mode "Classic".
 
 Ltac _red_tac c f term k :=
+  message 44;
+  message c;
+  message 55;
   match c with
   | inr ?c =>
-      (let tc := fresh "_TC_" in
-       unshelve evar (tc: @red_db c _ term);
-       [typeclasses eauto; instantiate (f:=_fail); fail|];
-       let lem := constr:(red_lemma tc) in
-       let _focused := constr:(red_focused tc) in
-       let focused := (eval simpl in _focused) in
-       let _next := constr:(red_next tc) in
-       let next := (eval simpl in _next) in
-       _red_tac next f focused ltac:(k; eapply lem))
+      tcsearch
+        (@red_db c _ term)
+        ltac:(fun tc =>
+                let lem := (eval red in (red_lemma tc)) in
+                let lem := (eval red in lem) in
+                let focused := (eval red in (red_focused tc)) in
+                let focused := (eval red in focused) in
+                let next := (eval red in (red_next tc)) in
+                let next := (eval red in next) in
+                (* message next; *)
+                (* message focused; *)
+                (* instantiate (f:=_break); *)
+                (* ltac:(k; apply lem)) *)
+                _red_tac next f focused ltac:(k; eapply lem))
   | inl ?fl =>
       instantiate (f:=fl); k
   end.
@@ -59,9 +95,6 @@ Ltac red_tac c f :=
       (_red_tac constr:(inr c: (_flag + red_class)%type) f term ltac:(idtac))
   end
 .
-
-Set Default Proof Mode "Classic".
-
 
 Module TUTORIAL.
   Section FOO.
@@ -90,27 +123,33 @@ Module TUTORIAL.
 
     Instance foo_red1_hint: red_db cl_A a :=
       mk_red_db _ _ foo_red0 b (inl _continue).
+
     Instance foo_red2_hint: red_db cl_A b :=
       mk_red_db _ _ foo_red1 c (inl _continue).
+
     Instance foo_red3_hint: red_db cl_B_unfold x :=
       mk_red_db _ _ foo_red3 y (inl _continue).
+
     Instance foo_red4_hint: red_db cl_B_unfold y :=
       mk_red_db _ _ foo_red4 y (inl _continue).
+
     Instance foo_red5_hint: red_db cl_C p :=
       mk_red_db _ _ foo_red5 q (inl _break).
+
     Instance cl_B_unfold_cl_B: red_db_incl cl_B_unfold cl_B := mk_red_db_incl.
 
     Instance foo_red_f_hint a: red_db cl_B (f a) :=
       mk_red_db _ _ (@f_equal _ _ f) a (inr cl_B).
 
-    Lemma foo: forall (n: nat) (H: sim c ((n, f z), q) n),
+    Goal forall (n: nat) (H: sim c ((n, f z), q) n),
         sim a ((n, f x), p) n.
     Proof.
       intros n H.
       (prw ltac:(red_tac cl_A) 3 0).
       (prw ltac:(red_tac cl_C) 2 1 0).
-      (prw ltac:(red_tac cl_B) 2 2 1 0).
+      (prw ltac:(red_tac cl_B) 2 2 1 1 0).
       exact H.
     Qed.
+
   End FOO.
 End TUTORIAL.
