src/lib/TCSearch.v
@@ -1,0 +1,30 @@
+From Ltac2 Require Import Ltac2.
+From Ltac2 Require Option Array Ident Control Std Fresh.
+
+Ltac2 or t0 t1 :=
+  match! 'True with
+  | True => t0 ()
+  | _ => t1 ()
+  end.
+
+Ltac2 fail () := Control.zero Match_failure.
+
+Ltac2 tcsearch e :=
+  let x := Array.make 1 constr:(tt: unit) in
+  or (fun _ =>
+        let n := Fresh.in_goal ident:(_TC_) in
+        ltac1:(e n|- unshelve evar (n: e);
+               [typeclasses eauto|]) (Ltac1.of_constr e) (Ltac1.of_ident n);
+        Array.set x 0 (Std.eval_unfold [(Std.VarRef n, Std.AllOccurrences)] (Control.hyp n));
+        fail ())
+     (fun _ => Array.get x 0)
+.
+
+Ltac tcsearch :=
+  ltac2:(e k |-
+           let e := Option.get (Ltac1.to_constr e) in
+           let v := tcsearch e in
+           Ltac1.apply k [Ltac1.of_constr v] Ltac1.run)
+.
+
+Set Default Proof Mode "Classic".
